Proof of basic valid judgement.

DlangLean/Sk.lean
@@ -10,48 +10,36 @@ inductive SkExpr where
 
 open SkExpr
 
-abbrev Context := List SkExpr
-
-def map_indices_free (n_binders : ℕ) (f : ℕ → ℕ) : SkExpr → SkExpr
-  | fall e_ty body => fall (map_indices_free n_binders.succ f e_ty) (map_indices_free n_binders.succ f body)
-  | t@(ty _) => t
-  -- if bound, don't touch this
-  | v@(var n) => if n ≥ n_binders then var (f n) else v
-  | x => x
-
-def substitute (with_expr : SkExpr) : SkExpr → SkExpr
+def substitute (n : ℕ) (with_expr : SkExpr): SkExpr → SkExpr
   | fall bind_ty body =>
-    let with_expr' := map_indices_free 0 (Nat.succ .) with_expr
-
-    fall (substitute with_expr' bind_ty) (substitute with_expr' body)
+    fall (substitute n.succ with_expr bind_ty) (substitute n.succ with_expr body)
   | t@(ty _) => t
-  | var 0 => with_expr
-  | var n => var $ n - 1
+  | var n' => if n == n' then with_expr else var $ n - 1
+  | call lhs rhs =>
+    call (substitute n with_expr lhs) (substitute n with_expr rhs)
+  | k => k
+  | s => s
+
+def body : SkExpr → SkExpr
+  | fall _ body => body
   | x => x
 
-inductive valid_judgement : Context → SkExpr → SkExpr → Prop
-  | k e t (h_is_k : match e with | SkExpr.k => true | _ => false) n m :
-    -- ∀ α β (x : α) (y : β), α
-    t = fall (SkExpr.ty n) (
-      fall (SkExpr.ty m) (
-        fall (SkExpr.var 0) (
-          fall (SkExpr.var 0) (SkExpr.var 3)))) → valid_judgement ctx e t
-  | s e t (h_is_s : match e with | SkExpr.s => true | _ => false) n m o :
+inductive valid_judgement : SkExpr → SkExpr → Prop
+  | k e t (h_is_k : match e with | SkExpr.k => true | _ => false) :
+    -- K α : ∀ β.∀ (x : α).∀ (y : β).α
+    t = fall (SkExpr.var 1) (
+          fall (SkExpr.var 1) (fall (SkExpr.var 3) (fall (SkExpr.var 3) (SkExpr.var 4)))) → valid_judgement e t
+  | s e t (h_is_s : match e with | SkExpr.s => true | _ => false) :
     -- ∀ α β γ (x : α → β → γ) (y : α → β) (z : α), γ
-    t = fall (SkExpr.ty n) (
-      fall (SkExpr.ty m) (
-        fall (SkExpr.ty o) (
-        fall (SkExpr.var 1) (
-          fall (SkExpr.var 1) (
-            fall (SkExpr.var 1) (
-              SkExpr.var 3)))))) → valid_judgement ctx e t
-  | call e t (lhs : SkExpr) (rhs : SkExpr) (t_rhs : SkExpr) (h_is_call : match e with | call _ _ => true | _ => false) :
-    valid_judgement ctx rhs t_rhs → valid_judgement (t_rhs :: ctx) (substitute lhs rhs) (fall t_rhs t) → valid_judgement ctx e t
+    t = fall (SkExpr.var 1) (
+          fall (SkExpr.var 1) (fall (SkExpr.var 1) (fall (SkExpr.var 4) (fall (SkExpr.var 4) (SkExpr.var 5))))) → valid_judgement e t
+  | call e t (lhs : SkExpr) (rhs : SkExpr) (t_lhs : SkExpr) (t_rhs : SkExpr) (h_is_call : match e with | call lhs' rhs' => lhs' = lhs ∧ rhs' = rhs | _ => false) :
+    valid_judgement lhs t_lhs → valid_judgement rhs t_rhs → t = body (substitute 0 rhs t_lhs) → valid_judgement e t
   | fall e t bind_ty body t_body (h_is_fall : match e with | fall _ _ => true | _ => false) :
-    valid_judgement ctx body t_body →
+    valid_judgement body t_body →
     e = fall bind_ty body →
-    t = t_body → valid_judgement ctx e t
-  | obvious e t : (match e with | ty n => t = ty (Nat.succ n) | var n => ctx[n]? = t | _ => false) → valid_judgement ctx e t
+    t = t_body → valid_judgement e t
+  | obvious e t : (match e with | ty n => t = ty n.succ | _ => false) → valid_judgement e t
 
 def eval_once : SkExpr → SkExpr
   | k => k
@@ -60,53 +48,30 @@ def eval_once : SkExpr → SkExpr
   | call (call (call s x) y) z => call (call x z) (call y z)
   | x => x
 
-def bruh := (call (call (call (call k (ty 1)) (ty 1)) (ty 0)) (ty 0))
-def is_valid_bruh : valid_judgement [] bruh (ty 1) :=
-  valid_judgement.call
-    bruh
+-- K α : ∀ β.∀ (x : α).∀ (y : β).α
+example : valid_judgement (call k (ty 1)) (fall (var 1) (fall (ty 1) (fall (var 3) (ty 1)))) := by
+  apply (valid_judgement.call
+    -- e
+    (call k (ty 1))
+    -- t
+    (fall (var 1) (fall (ty 1) (fall (var 3) (ty 1))))
+    -- lhs
+    k
+    -- rhs
     (ty 1)
-    (call (call (call k (ty 1)) (ty 1)) (ty 0))
-    (ty 0)
-    (ty 1)
-    (by unfold bruh; simp)
-    (valid_judgement.obvious
-      (ty 0)
-      (ty 1)
-      (by simp))
-    (valid_judgement.call
-      (substitute (((k.call (ty 1)).call (ty 1)).call (ty 0)) (ty 0))
-      (call (call (call k (ty 1)) (ty 1)) (ty 0))
-      ((ty 1).fall (ty 1))
-      (call (call k (ty 1)) (ty 1))
-      (ty 0)
-      (ty 1)
-      (by simp)
-      (valid_judgement.obvious (ty 0) (ty 1) (by simp))
-      (@valid_judgement.call []
-        ((k.call (ty 1)).call (ty 1))
-        ((ty 1).fall ((ty 1).fall (ty 1)))
-        (k.call (ty 1))
-        (ty 1)
-        (ty 2)
-        (by simp_all)
-        (valid_judgement.obvious (ty 1) (ty 2) (by simp))
-        (@valid_judgement.call
-          []
-          (k.call (ty 1))
-          ((ty 2).fall ((ty 1).fall ((ty 1).fall (ty 1))))
-          k
-          (ty 1)
-          (ty 2)
-          (by simp)
-          (valid_judgement.obvious (ty 1) (ty 2) (by simp))
-          (@valid_judgement.k [] k
-            ((ty 2).fall ((ty 2).fall ((var 0).fall ((var 0).fall (var 3)))))
-            (by simp)
-            2
-            2
-            rfl
-          )
-        )
-      ))
+    -- t_lhs
+    (fall (SkExpr.var 1) (
+          fall (SkExpr.var 1) (fall (SkExpr.var 3) (fall (SkExpr.var 3) (SkExpr.var 4)))))
+    -- t_rhs
+    (ty 2)
+    (by simp)
+  )
+  simp [valid_judgement.k]
+  simp [valid_judgement.obvious]
+  unfold substitute
+  simp
+  repeat unfold substitute
+  simp
+  unfold body
+  simp
 
-#eval valid_judgement [] 
